extraction/examples/RustCounter.v
@@ -1,0 +1,53 @@
+From Coq Require Import String.
+From Coq Require Import ZArith.
+From Coq Require Import Bool.
+
+From ConCert.Extraction Require Import RustExtract.
+From ConCert.Extraction Require Import Common.
+From ConCert.Extraction Require Import ConcordiumExtract.
+From ConCert.Extraction Require Import ResultMonad.
+
+From ConCert.Extraction.Examples Require Import CounterRefinementTypes.
+From MetaCoq.Template Require Import All.
+
+Import MonadNotation.
+
+Module C := CounterRefinementTypes.
+
+Open Scope string.
+
+Instance RustCounterConfig : RustPrintConfig :=
+  {| term_box_symbol := "()";
+     type_box_symbol := "()";
+     any_type_symbol := "()";
+     print_full_names := false |}.
+
+Definition remap_blockchain : list (kername * string) := Eval compute in
+      [ remap <%% C.Transaction  %%> "type Transaction<'a> = ();"
+      ; remap <%% C.Transaction_none %%> "fn ##name## (&'a self) -> Transaction<'a> { () }" ].
+
+(* TODO: remap <%% nat %%> "AccountAddress" *)
+
+Time MetaCoq Run
+     (r <- tmQuoteRecTransp CounterRefinementTypes.counter false;;
+      tmDefinition "COUNTER" r
+     ).
+
+MetaCoq Quote Recursively Definition blah := bool_rect.
+
+Definition counter_result:=
+  Eval vm_compute in extract COUNTER
+                             (ConcordiumRemap.build_remaps
+                                (ConcordiumRemap.remap_arith ++ remap_blockchain)
+                                []
+                                (ConcordiumRemap.remap_std_types))
+                             (fun kn => eq_kername <%% bool_rec %%> kn
+                                     || eq_kername <%% bool_rect %%> kn).
+
+Definition rust_counter :=
+  match counter_result with
+  | Ok v => tmMsg v
+  | Err e => tmFail e
+  end.
+
+MetaCoq Run rust_counter.
