extraction/theories/ConcordiumExtract.v
@@ -1,0 +1,232 @@
+From MetaCoq Require Import monad_utils.
+From MetaCoq Require Import utils.
+From MetaCoq.Template Require Import All.
+From MetaCoq.Template Require Import Kernames.
+
+From ConCert.Extraction Require Import Common.
+From ConCert.Extraction Require Import Extraction.
+From ConCert.Extraction Require Import RustExtract.
+From ConCert.Extraction Require Import Optimize.
+From ConCert.Extraction Require Import PrettyPrinterMonad.
+From ConCert.Extraction Require Import Printing.
+From ConCert.Extraction Require Import ResultMonad.
+From ConCert.Extraction Require Import Utils.
+From ConCert.Extraction.Examples Require Import CounterRefinementTypes.
+From ConCert.Extraction.Examples Require Import RustExtractTests.
+From ConCert.Utils Require Import StringExtra.
+
+Module ConcordiumRemap.
+
+Definition lookup_const (TT : list (kername * string)) (name : kername): option string :=
+  match find (fun '(key, _) => eq_kername key name) TT with
+  | Some (_, val) => Some val
+  | None => None
+  end.
+
+Definition remap_arith : list (kername * string) := Eval compute in
+  [  remap <%% BinPosDef.Pos.add %%> "fn ##name##(&'a self, a: u64, b: u64) -> u64 { a.checked_add(b).unwrap() }"
+   ; remap <%% BinPosDef.Pos.succ %%> "fn ##name##(&'a self, a: u64) -> u64 { a.checked_add(1).unwrap() }"
+   ; remap <%% Z.add %%> "fn ##name##(&'a self, a: i64, b: i64) -> i64 { a.checked_add(b).unwrap() }"
+   ; remap <%% Z.sub %%> "fn ##name##(&'a self, a: i64, b: i64) -> i64 { a.checked_sub(b).unwrap() }"
+  ; remap <%% Z.leb %%> "fn ##name##(&'a self, a: i64, b: i64) -> bool { a <= b }"
+  ; remap <%% Z.ltb %%> "fn ##name##(&'a self, a: i64, b: i64) -> bool { a < b }" ].
+
+Definition remap_positive : remapped_inductive :=
+  {| re_ind_name := "u64";
+     re_ind_ctors := ["__pos_onebit"; "__pos_zerobit"; "1"];
+     re_ind_match := None
+  |}.
+
+Definition remap_Z : remapped_inductive :=
+  {| re_ind_name := "i64";
+     re_ind_ctors := ["0"; "__Z_frompos"; "__Z_fromneg"];
+     re_ind_match := None
+  |}.
+
+Definition remap_bool : remapped_inductive :=
+  {| re_ind_name := "bool";
+     re_ind_ctors := ["true"; "false"];
+     re_ind_match := None
+  |}.
+
+
+Definition remap_pair : remapped_inductive :=
+  {| re_ind_name := "__pair";
+     re_ind_ctors := ["__mk_pair"];
+     re_ind_match := Some "__pair_elim"
+  |}.
+
+Definition remap_std_types :=
+  [ (<%% positive %%>, remap_positive)
+  ; (<%% Z %%>,  remap_Z)
+  ; (<%% bool %%>, remap_bool)
+  ; (<%% prod %%>, remap_pair)].
+
+Definition lookup_inductive (TT_inductives : list (kername * remapped_inductive))  (ind : inductive) : option remapped_inductive :=
+  match find (fun '(key, _) => eq_kername key (inductive_mind ind)) TT_inductives with
+  | Some (_, val) => Some val
+  | None => None
+  end.
+
+Definition build_remaps
+           (TT_const : list (kername * string))
+           (TT_const_inline : list (kername * string))
+           (TT_inductives : list (kername * remapped_inductive))
+  : remaps :=
+  {| remap_inductive := lookup_inductive TT_inductives;
+     remap_constant := lookup_const TT_const;
+     remap_inline_constant := lookup_const TT_const_inline; |}.
+
+End ConcordiumRemap.
+
+Module ConcordiumPreamble.
+  Instance concordium_extract_preamble : Preamble :=
+{| top_preamble := [
+"#![allow(dead_code)]";
+"#![allow(non_camel_case_types)]";
+"#![allow(unused_imports)]";
+"#![allow(non_snake_case)]";
+"#![allow(unused_variables)]";
+ "";
+"use concordium_std::*;";
+"use core::marker::PhantomData;";
+"";
+"fn __nat_succ(x: u64) -> u64 {";
+"  x.checked_add(1).unwrap()";
+"}";
+"";
+"macro_rules! __nat_elim {";
+"    ($zcase:expr, $pred:ident, $scase:expr, $val:expr) => {";
+"        { let v = $val;";
+"        if v == 0 { $zcase } else { let $pred = v - 1; $scase } }";
+"    }";
+"}";
+"";
+"macro_rules! __andb { ($b1:expr, $b2:expr) => { $b1 && $b2 } }";
+"macro_rules! __orb { ($b1:expr, $b2:expr) => { $b1 || $b2 } }";
+"";
+"fn __pos_onebit(x: u64) -> u64 {";
+"  x.checked_mul(2).unwrap() + 1";
+"}";
+"";
+"fn __pos_zerobit(x: u64) -> u64 {";
+"  x.checked_mul(2).unwrap()";
+"}";
+"";
+"macro_rules! __pos_elim {";
+"    ($p:ident, $onebcase:expr, $p2:ident, $zerobcase:expr, $onecase:expr, $val:expr) => {";
+"        {";
+"            let n = $val;";
+"            if n == 1 {";
+"                $onecase";
+"            } else if (n & 1) == 0 {";
+"                let $p2 = n >> 1;";
+"                $zerobcase";
+"            } else {";
+"                let $p = n >> 1;";
+"                $onebcase";
+"            }";
+"        }";
+"    }";
+"}";
+"";
+"fn __Z_frompos(z: u64) -> i64 {";
+"  use std::convert::TryFrom;";
+"";
+"  i64::try_from(z).unwrap()";
+"}";
+"";
+"fn __Z_fromneg(z : u64) -> i64 {";
+"  use std::convert::TryFrom;";
+"";
+"  i64::try_from(z).unwrap().checked_neg().unwrap()";
+"}";
+"";
+"macro_rules! __Z_elim {";
+"    ($zero_case:expr, $p:ident, $pos_case:expr, $p2:ident, $neg_case:expr, $val:expr) => {";
+"        {";
+"            let n = $val;";
+"            if n == 0 {";
+"                $zero_case";
+"            } else if n < 0 {";
+"                let $p2 = n.unsigned_abs();";
+"                $neg_case";
+"            } else {";
+"                let $p = n as u64;";
+"                $pos_case";
+"            }";
+"        }";
+"    }";
+"}";
+"";
+"fn __N_frompos(z: u64) -> u64 {";
+"  z";
+"}";
+"";
+"macro_rules! __N_elim {";
+"    ($zero_case:expr, $p:ident, $pos_case:expr, $val:expr) => {";
+"        { let $p = $val; if $p == 0 { $zero_case } else { $pos_case } }";
+"    }";
+"}";
+"";
+"type __pair<A, B> = (A, B);";
+"";
+"macro_rules! __pair_elim {";
+"    ($fst:ident, $snd:ident, $body:expr, $p:expr) => {";
+"        { let ($fst, $snd) = $p; $body }";
+"    }";
+"}";
+"";
+"fn __mk_pair<A: Copy, B: Copy>(a: A, b: B) -> __pair<A, B> { (a, b) }";
+"";
+"fn hint_app<TArg, TRet>(f: &dyn Fn(TArg) -> TRet) -> &dyn Fn(TArg) -> TRet {";
+"  f";
+"}" ];
+program_preamble := [
+"fn alloc<T>(&'a self, t: T) -> &'a T {";
+"  self.__alloc.alloc(t)";
+"}";
+"";
+"fn closure<TArg, TRet>(&'a self, F: impl Fn(TArg) -> TRet + 'a) -> &'a dyn Fn(TArg) -> TRet {";
+"  self.__alloc.alloc(F)";
+"}" ] |}.
+
+End ConcordiumPreamble.
+
+Import ConcordiumRemap.
+
+Definition extract_lines
+           (p : T.program)
+           (remaps : remaps)
+           (should_inline : kername -> bool) : result (list string) string :=
+  entry <- match p.2 with
+           | T.tConst kn _ => ret kn
+           | T.tInd ind _ => ret (inductive_mind ind)
+           | _ => Err "Expected program to be a tConst or tInd"
+           end;;
+  let without_deps kn :=
+      if remap_inductive remaps (mkInd kn 0) then true else
+      if remap_constant remaps kn then true else
+      if remap_inline_constant remaps kn then true else false in
+  Σ <- extract_template_env
+         (extract_rust_within_coq should_inline)
+         p.1
+         (KernameSet.singleton entry)
+         without_deps;;
+  let p :=
+      names <- print_program Σ remaps;;
+
+      (* TODO: replace with something else from the Concordium infrastructure *)
+      append_nl;;
+      append "fn main() {";;
+      append_nl;;
+      let name := const_global_ident_of_kername entry in
+      append ("  print!(""{:?}"", Program::new()." ++ name ++ "())");;
+      append_nl;;
+      append "}" in
+  '(_, s) <- timed "Printing" (fun _ => finish_print_lines p);;
+  ret s.
+
+Definition extract p remaps should_inline :=
+  lines <- extract_lines p remaps should_inline;;
+  ret (String.concat nl lines).
