extraction/theories/PluginExtract.v
@@ -1,0 +1,167 @@
+(** * Definitions below are used in the extracted plugin *)
+
+From ConCert.Extraction Require Import Common.
+From ConCert.Extraction Require Import Erasure.
+From ConCert.Extraction Require Import ExAst.
+From ConCert.Extraction Require Import ExpandBranches.
+From ConCert.Extraction Require Import Extraction.
+From ConCert.Extraction Require Import Inlining.
+From ConCert.Extraction Require Import Optimize.
+From ConCert.Extraction Require Import PrettyPrinterMonad.
+From ConCert.Extraction Require Import Printing.
+From ConCert.Extraction Require Import ResultMonad.
+From ConCert.Extraction Require Import TopLevelFixes.
+From ConCert.Extraction Require Import Utils.
+From ConCert.Extraction Require Import RustExtract.
+From MetaCoq.Template Require Import Kernames.
+
+Instance plugin_extract_preamble : Preamble :=
+{| top_preamble := [
+"#![allow(dead_code)]";
+"#![allow(non_camel_case_types)]";
+"#![allow(unused_imports)]";
+"#![allow(non_snake_case)]";
+"#![allow(unused_variables)]";
+"#![feature(unsigned_abs)]";
+"";
+"use std::marker::PhantomData;";
+"";
+"fn __nat_succ(x: u64) -> u64 {";
+"  x.checked_add(1).unwrap()";
+"}";
+"";
+"macro_rules! __nat_elim {";
+"    ($zcase:expr, $pred:ident, $scase:expr, $val:expr) => {";
+"        { let v = $val;";
+"        if v == 0 { $zcase } else { let $pred = v - 1; $scase } }";
+"    }";
+"}";
+"";
+"macro_rules! __andb { ($b1:expr, $b2:expr) => { $b1 && $b2 } }";
+"macro_rules! __orb { ($b1:expr, $b2:expr) => { $b1 || $b2 } }";
+"";
+"fn __pos_onebit(x: u64) -> u64 {";
+"  x.checked_mul(2).unwrap() + 1";
+"}";
+"";
+"fn __pos_zerobit(x: u64) -> u64 {";
+"  x.checked_mul(2).unwrap()";
+"}";
+"";
+"macro_rules! __pos_elim {";
+"    ($p:ident, $onebcase:expr, $p2:ident, $zerobcase:expr, $onecase:expr, $val:expr) => {";
+"        {";
+"            let n = $val;";
+"            if n == 1 {";
+"                $onecase";
+"            } else if (n & 1) == 0 {";
+"                let $p2 = n >> 1;";
+"                $zerobcase";
+"            } else {";
+"                let $p = n >> 1;";
+"                $onebcase";
+"            }";
+"        }";
+"    }";
+"}";
+"";
+"fn __Z_frompos(z: u64) -> i64 {";
+"  use std::convert::TryFrom;";
+"";
+"  i64::try_from(z).unwrap()";
+"}";
+"";
+"fn __Z_fromneg(z : u64) -> i64 {";
+"  use std::convert::TryFrom;";
+"";
+"  i64::try_from(z).unwrap().checked_neg().unwrap()";
+"}";
+"";
+"macro_rules! __Z_elim {";
+"    ($zero_case:expr, $p:ident, $pos_case:expr, $p2:ident, $neg_case:expr, $val:expr) => {";
+"        {";
+"            let n = $val;";
+"            if n == 0 {";
+"                $zero_case";
+"            } else if n < 0 {";
+"                let $p2 = n.unsigned_abs();";
+"                $neg_case";
+"            } else {";
+"                let $p = n as u64;";
+"                $pos_case";
+"            }";
+"        }";
+"    }";
+"}";
+"";
+"fn __N_frompos(z: u64) -> u64 {";
+"  z";
+"}";
+"";
+"macro_rules! __N_elim {";
+"    ($zero_case:expr, $p:ident, $pos_case:expr, $val:expr) => {";
+"        { let $p = $val; if $p == 0 { $zero_case } else { $pos_case } }";
+"    }";
+"}";
+"";
+"type __pair<A, B> = (A, B);";
+"";
+"macro_rules! __pair_elim {";
+"    ($fst:ident, $snd:ident, $body:expr, $p:expr) => {";
+"        { let ($fst, $snd) = $p; $body }";
+"    }";
+"}";
+"";
+"fn __mk_pair<A: Copy, B: Copy>(a: A, b: B) -> __pair<A, B> { (a, b) }";
+"";
+"fn hint_app<TArg, TRet>(f: &dyn Fn(TArg) -> TRet) -> &dyn Fn(TArg) -> TRet {";
+"  f";
+"}" ];
+program_preamble := [
+"fn alloc<T>(&'a self, t: T) -> &'a T {";
+"  self.__alloc.alloc(t)";
+"}";
+"";
+"fn closure<TArg, TRet>(&'a self, F: impl Fn(TArg) -> TRet + 'a) -> &'a dyn Fn(TArg) -> TRet {";
+"  self.__alloc.alloc(F)";
+"}" ] |}.
+
+Instance RustConfig : RustPrintConfig :=
+  {| term_box_symbol := "()";
+     type_box_symbol := "()";
+     any_type_symbol := "()";
+     print_full_names := true |}.
+
+Definition extract_lines
+           (p : T.program)
+           (remaps : remaps)
+           (should_inline : kername -> bool) : result (list string) string :=
+  entry <- match p.2 with
+           | T.tConst kn _ => ret kn
+           | T.tInd ind _ => ret (inductive_mind ind)
+           | _ => Err "Expected program to be a tConst or tInd"
+           end;;
+  let without_deps kn :=
+      if remap_inductive remaps (mkInd kn 0) then true else
+      if remap_constant remaps kn then true else
+      if remap_inline_constant remaps kn then true else false in
+  Σ <- extract_template_env
+         (extract_rust_within_coq should_inline)
+         p.1
+         (KernameSet.singleton entry)
+         without_deps;;
+  let p :=
+      names <- print_program Σ remaps;;
+      append_nl;;
+      append "fn main() {";;
+      append_nl;;
+      let name := const_global_ident_of_kername entry in
+      append ("  print!(""{:?}"", Program::new()." ++ name ++ "())");;
+      append_nl;;
+      append "}" in
+  '(_, s) <- timed "Printing" (fun _ => finish_print_lines p);;
+  ret s.
+
+Definition extract p remaps should_inline :=
+  lines <- extract_lines p remaps should_inline;;
+  ret (String.concat nl lines).
